bootstrapQ
git-svn-id: svn://scm.gforge.inria.fr/svn/cfml@20 ba02c806-7d2b-4818-9a48-35b22e6bdc79

okasaki/AltBinaryRandomAccessList.ml
@@ -1,24 +1,23 @@
 open Okasaki
 open RandomAccessListSig
 
-(*
 module AltBinaryRandomAccesList : RandomAccessList =
 struct
 
    type 'a rlist = Nil | Zero of ('a * 'a) rlist | One of 'a * ('a * 'a) rlist
 
-   let empty : 'a rlist = Nil
+   let empty = Nil
 
    let is_empty = function  
       | Nil -> true
       | _ -> false
 
-   let rec cons : 'a -> 'a rlist -> 'a rlist = fun x -> function
+   let rec cons : 'a. 'a -> 'a rlist -> 'a rlist = fun x -> function
       | Nil -> One (x, Nil)
       | Zero ps -> One (x, ps)
       | One (y, ps) -> Zero (cons (x,y) ps)
 
-   let rec uncons : 'a rlist -> 'a * 'a rlist = function
+   let rec uncons : 'a. 'a rlist -> 'a * 'a rlist = function
       | Nil -> raise EmptyStructure
       | One (x, Nil) -> (x, Nil)
       | One (x, ps) -> (x, Zero ps)
@@ -32,7 +31,7 @@ struct
    let tail ts = 
       snd (uncons ts)
 
-   let rec lookup i ts = 
+   let rec lookup : 'a. int -> 'a rlist -> 'a = fun i ts ->
       match i,ts with
       | i, Nil -> raise OutOfBound
       | 0, One (x, ps) -> x
@@ -41,7 +40,7 @@ struct
          let (x,y) = lookup (i/2) ps in
          if i mod 2 = 0 then x else y
 
-   let rec fupdate f i ts = 
+   let rec fupdate f i ts : 'a. ('a -> 'a) -> int -> 'a rlist -> 'a rlist = 
       match i,ts with
       | i, Nil -> raise OutOfBound
       | 0, One (x, ps) -> One (f x, ps)
@@ -50,8 +49,7 @@ struct
          let f' (x,y) = if i mod 2 = 0 then (f x, y) else (x, f y) in
          Zero (fupdate f' (i/2) ps)
                       
-   let update i y xs = fupdate (fun x -> (y,i,xs))
+   let update i y xs = fupdate (fun x -> y) i xs
 
 end
 
-*)
