okasaki/HoodMelvilleQueue.ml
@@ -1,6 +1,5 @@
 open Okasaki
 open QueueSig
-(* todo: bug des variables nommées comme les types *)
 
 module HoodMelvilleQueue : Queue = struct
 
@@ -25,22 +24,22 @@ module HoodMelvilleQueue : Queue = struct
      | Appending (ok, f', r') -> Appending (ok-1, f', r')
      | s -> s
 
-   let exec2 (lenf,f,state,lenr,r) = 
+   let exec2 (lenf, f, state, lenr, r) = 
      match exec (exec state) with
      | Done newf -> (lenf, newf, Idle, lenr, r)
      | newstate -> (lenf, f, newstate, lenr, r)
 
-   let check ((lenf,f,state,lenr,r) as q) = 
+   let check ((lenf, f, state, lenr, r) as q) = 
      if lenr <= lenf 
         then exec2 q                         
-        else let newstate = Reversing (0,f,[],r,[]) in
-             exec2 (lenf+lenr,f,newstate,0,[])
+        else let newstate = Reversing (0, f, [], r, []) in
+             exec2 (lenf+lenr, f, newstate, 0, [])
 
-   let empty = (0,[],Idle,0,[])
+   let empty = (0, [], Idle, 0, [])
 
    let is_empty (lenf, _, _, _, _) = (lenf = 0)
 
-   let snoc (lenf,f,state,lenr,r) x =
+   let snoc (lenf, f, state, lenr, r) x =
       check (lenf, f, state, lenr+1, x::r)
       
    let head = function
@@ -49,7 +48,8 @@ module HoodMelvilleQueue : Queue = struct
 
    let tail = function 
      | (_,[],_,_,_) -> raise EmptyStructure
-     | (lenf,x::f',state,lenr,r) -> check (lenf-1,f',invalidate state,lenr,r)
+     | (lenf, x::f', state, lenr, r) ->
+        check (lenf-1, f', invalidate state, lenr, r)
 
 end
 
