okasaki/PhysicistsQueue_proof.v
@@ -101,12 +101,6 @@ Qed.
 
 Hint Extern 1 (RegisterSpec check) => Provide check_spec.
 
-(* todo: move *)
-Lemma app_rev_cons : forall A (x:A) l1 l2,
-  l1 ++ rev (x :: l2) = (l1 ++ rev l2) & x.
-Proof. intros. rewrite rev_cons. rewrite~ app_assoc. Qed.
-
-
 Lemma snoc_spec : 
   RepTotal snoc (Q;queue a) (X;a) >> (Q & X) ; queue a.
 Proof.
@@ -119,7 +113,7 @@ Hint Extern 1 (RegisterSpec snoc) => Provide snoc_spec.
 
 Lemma head_spec : 
   RepSpec head (Q;queue a) |R>>
-     Q <> (@nil A) -> R (is_head Q ;; a).
+     Q <> nil -> R (is_head Q ;; a).
 Proof.
   xcf. intros ((((w,lenf),f),lenr),r) Q RQ NE.
   forwards*: rep_not_nil. destruct Q. false. intuit RQ.
