okasaki/RealTimeQueue_proof.v
@@ -113,7 +113,7 @@ Hint Extern 1 (RegisterSpec snoc) => Provide snoc_spec.
 
 Lemma head_spec : 
   RepSpec head (Q;queue a_) |R>>
-     Q <> (@nil A) -> R (is_head Q ;; a_).
+     Q <> nil -> R (is_head Q ;; a_).
 Proof.
   xcf. intros ((f,r),s) Q. introv RQ NE. xgo.
   false (repr_nil_inv RQ).
